local build fixed

src/Init/Data/BitVec/Basic.lean
@@ -872,17 +872,16 @@ def clz (x : BitVec w) : BitVec w := clzAuxRec x (w - 1)
 /-- Count the number of trailing zeros. -/
 def ctz (x : BitVec w) : BitVec w := (x.reverse).clz
 
-/-- Count the number of bits with value `1` downward from the `pos`-th bit to the
-  `0`-th bit of `x`, storing the result in `acc`. -/
-def cpopNatRec (x : BitVec w) (pos acc : Nat) : Nat :=
-  match pos with
-  | 0 => acc
-  | n + 1 => x.cpopNatRec n (acc + (x.getLsbD n).toNat)
+/-- Tail-recursive definition of popcount.
+ The bitwidth of `x` explictly boundspop the number of recursions,
+ thus bounding the depth of the circuit as well correctness of def -/
+def popCountAuxRec (x : BitVec w) (r : BitVec v) (n : Nat) :=
+  match h : (w - n) with
+  | 0 => r
+  | n' + 1 => x.popCountAuxRec (r + (x.extractLsb' n 1).zeroExtend v) (n + 1)
+termination_by (w - n)
 
-/-- Population count operation, to count the number of bits with value `1` in `x`.
-  Also known as `popcount`, `popcnt`.
--/
-@[suggest_for BitVec.popcount BitVec.popcnt]
-def cpop (x : BitVec w) : BitVec w := BitVec.ofNat w (cpopNatRec x w 0)
+/-- Count the number of bits with value `1` in a bitvec -/
+def popCount {w : Nat} (x : BitVec w) : BitVec w := BitVec.popCountAuxRec x 0#w 0
 
 end BitVec
