src/Std/Tactic/BVDecide/Bitblast/BVExpr/Circuit/Impl/Expr.lean
@@ -232,6 +232,12 @@ where
           apply AIG.LawfulVecOperator.le_size_of_le_aig_size (f := bitblast.blastClz)
           omega
         ⟨⟨res, this⟩, cache.cast (AIG.LawfulVecOperator.le_size (f := bitblast.blastClz) ..)⟩
+      | .popCount =>
+        let res := bitblast.blastPopCount eaig evec
+        have := by
+          apply AIG.LawfulVecOperator.le_size_of_le_aig_size (f := bitblast.blastPopCount)
+          omega
+        ⟨⟨res, this⟩, cache.cast (AIG.LawfulVecOperator.le_size (f := bitblast.blastPopCount) ..)⟩
     | .append lhs rhs h =>
       let ⟨⟨⟨aig, lhs⟩, hlaig⟩, cache⟩ := goCache aig lhs cache
       let ⟨⟨⟨aig, rhs⟩, hraig⟩, cache⟩ := goCache aig rhs cache
@@ -343,7 +349,7 @@ theorem go_decl_eq (aig : AIG BVBit) (expr : BVExpr w) (cache : Cache aig) :
         · apply Nat.le_trans <;> assumption
   next op expr =>
     match op with
-    | .not | .rotateLeft .. | .rotateRight .. | .arithShiftRightConst .. | .reverse | .clz =>
+    | .not | .rotateLeft .. | .rotateRight .. | .arithShiftRightConst .. | .reverse | .clz | .popCount =>
       rw [AIG.LawfulVecOperator.decl_eq]
       rw [goCache_decl_eq]
       have := (goCache aig expr cache).result.property
